New scala implementation

Isabelle2/MultiPaxos4.thy
@@ -42,8 +42,6 @@ datatype 'v msg =
 | Phase1b (last_votes:"inst \<Rightarrow>f (bal \<times> ('v cmd option))") (new_ballot: bal) (acceptor:acc)
 | Phase2a (inst: inst) (for_ballot:bal) (suggestion:"'v cmd") (leader: acc)
 | Phase2b (inst: inst) (ballot:bal) (acceptor: acc) (cmd: "'v cmd")
-| Vote (inst: inst) (cmd: "'v cmd")
-  -- {* Instructs a learner that a value has been decided. Not used for now... *}
 | Fwd (val: 'v)
   -- {* Forwards a proposal to another proposer (the leader) *}
 
@@ -52,7 +50,9 @@ datatype 'v packet =
   Packet (sender: acc) (dst: acc) (msg: "'v msg")
 
 record 'v acc_state =
+  id :: "acc"
   leader :: "bool"
+  acceptors :: "acc fset"
 
   ballot :: "bal"
   decided :: "inst \<Rightarrow>f 'v cmd option"
@@ -61,22 +61,22 @@ record 'v acc_state =
     -- {* The last vote cast by an acceptor, for each instance *}
   last_ballot :: "inst \<Rightarrow>f bal"
     -- {* For an acceptor a, this is the ballot in which "vote a" was cast, for each instance *}
-  onebs :: "bal \<Rightarrow>f inst \<Rightarrow>f (acc \<times> bal \<times> ('v cmd option)) set"
+  onebs :: "bal \<Rightarrow>f inst \<Rightarrow>f (acc \<times> bal \<times> ('v cmd option)) list"
     -- {* For an acceptor a and a ballot b, lists of 1b-message descriptions, indexed by ballot then instance. *}
-  twobs :: "inst \<Rightarrow>f bal \<Rightarrow>f acc set"
+  twobs :: "inst \<Rightarrow>f bal \<Rightarrow>f acc list"
     -- {* For an acceptor a: lists describing the 2b messages, indexed by instance then ballot. *}
 
   next_inst :: "inst"
-  working_instances :: "inst \<Rightarrow>f nat" 
+  status :: "inst \<Rightarrow>f nat" 
     -- {* 0: not started; 1: processing; 2: closed *}
   
 fun accs where
   "accs (0::nat) = {||}"
 | "accs (Suc n) = (accs n) |\<union>| {|n|}"
 
-definition nr where
+definition nas where
   -- {* The number of replicas *}
-  "nr acceptors \<equiv> card acceptors"
+  "nas s \<equiv> fcard (acceptors s)"
 
 text {* A few functions to export to Scala for use by the runtime. *}
 
@@ -85,32 +85,34 @@ definition get_ballot where "get_ballot s \<equiv> ballot s"
 definition is_leader where "is_leader s \<equiv> leader s"
 
 definition get_leader where 
-  "get_leader s nas \<equiv> case ballot s of 0 \<Rightarrow> None | b \<Rightarrow> Some (b mod nas)"
+  "get_leader s \<equiv> case ballot s of 0 \<Rightarrow> None | b \<Rightarrow> Some (b mod (nas s))"
 
 definition get_next_instance where
   "get_next_instance s \<equiv> next_inst s"
 
-definition init_acc_state :: "'v acc_state" where
-  "init_acc_state \<equiv> \<lparr>
+definition init_acc_state :: "nat \<Rightarrow> acc \<Rightarrow> 'v acc_state" where
+  "init_acc_state n a \<equiv> \<lparr>
+    id = a,
     leader = False,
+    acceptors = accs n,
 
     ballot = 0,
     decided = K$ None,
     vote = K$ None, 
     last_ballot = K$ 0,
-    onebs = K$ K$ {},
-    twobs = K$ K$ {},
+    onebs = K$ K$ [],
+    twobs = K$ K$ [],
 
     next_inst = 1, (* instances start at 1 *)
-    working_instances =  K$ 0
+    status =  K$ 0
    \<rparr>" 
 
 text {* If we had finfun_Ex we could do this better.
   Here we use instance 0 by default, but that's arbitrary. *}
 definition one_b_quorum_received where
-  "one_b_quorum_received b s nas \<equiv> 
+  "one_b_quorum_received b s \<equiv> 
     let at_b_i = onebs s $ b $ 0
-    in 2 * card at_b_i > nas"
+    in 2 * length at_b_i > (nas s)"
 
 fun getOwnedBallot where 
   "getOwnedBallot a (Suc b) N = (if ((Suc b) mod N = a) then (Suc b)
@@ -122,49 +124,45 @@ definition suc_bal :: "nat \<Rightarrow> nat \<Rightarrow> nat \<Rightarrow> nat
   where "suc_bal a b N \<equiv> getOwnedBallot a (b + N) N"
 
 definition leader_of_bal::"nat \<Rightarrow> nat \<Rightarrow> nat" where
-  "leader_of_bal b nas \<equiv> case b of 0 \<Rightarrow> 0 | bs \<Rightarrow> (bs mod nas)"
+  "leader_of_bal b n \<equiv> case b of 0 \<Rightarrow> 0 | bs \<Rightarrow> (bs mod n)"
                                    
-definition send_all where "send_all acc ms acceptors \<equiv> fimage (\<lambda> a2 . Packet acc a2 ms)  (acceptors |-| {|acc|})"
+definition send_all where "send_all acc mesg s \<equiv> fimage (\<lambda> a2 . Packet acc a2 mesg) (acceptors s |-| {|acc|})"
 
 definition do_2a where
-  "do_2a a s v acceptors \<equiv>
+  "do_2a a s v \<equiv>
     let
       inst = (next_inst s);
       b = (ballot s);
       msg = Phase2a inst b v a;
       new_state = s\<lparr>next_inst := (inst + 1),
-        twobs := (twobs s)(inst $:= ((twobs s $ inst)(b $:= {a}))),
-        working_instances := (working_instances s)(inst $:= 1) (* Added by ian to track working instances *)
+        twobs := (twobs s)(inst $:= ((twobs s $ inst)(b $:= [a]))),
+        status := (status s)(inst $:= 1) (* Added by ian to track working instances *)
        \<rparr>
     in
-      (new_state, send_all a msg acceptors)"
+      (new_state, send_all a msg s)"
 
-definition propose :: "acc \<Rightarrow> 'v \<Rightarrow> 'v acc_state \<Rightarrow> nat \<Rightarrow> acc fset \<Rightarrow> ('v acc_state \<times> 'v packet fset)" where
+definition propose :: "acc \<Rightarrow> 'v \<Rightarrow> 'v acc_state \<Rightarrow> ('v acc_state \<times> 'v packet fset)" where
   -- {* If leader, then go ahead with 2a, otherwise forward to the leader. *}
-  "propose a v s nas acceptors \<equiv> let leader_bal = (leader_of_bal (ballot s) nas) 
-    in
-    (if (leader_bal = a \<and> leader s)
-      then do_2a a s (Cmd v) acceptors
-      else (if (leader_bal = a)
-        then (s,{||}) (* TODO: here we loose the proposal... *)
-        else (s, {|Packet a leader_bal (Fwd v)|})))"
+  "propose a v s \<equiv> (if (leader s)
+      then (do_2a a s (Cmd v))
+      else (s, {|Packet a (leader_of_bal (ballot s) (nas s)) (Fwd v)|}))"
  
 (* What if the target process is not the leader anymore? TODO: Then let's forward it again. *)
-definition receive_fwd  :: "acc \<Rightarrow> 'v \<Rightarrow> 'v acc_state \<Rightarrow> nat \<Rightarrow> acc fset \<Rightarrow> ('v acc_state \<times> 'v packet fset)" where
-  "receive_fwd a v s nas acceptors \<equiv>
-    (if (leader_of_bal (ballot s) nas = a \<and> leader s) then do_2a a s (Cmd v) acceptors else (s, {||}))"
+definition receive_fwd  :: "'v \<Rightarrow> 'v acc_state \<Rightarrow> ('v acc_state \<times> 'v packet fset)" where
+  "receive_fwd v s \<equiv> (let a = id s in
+    (if (leader_of_bal (ballot s) (nas s) = a \<and> leader s) then do_2a a s (Cmd v) else (s, {||})))"
 
-definition send_1a :: "acc \<Rightarrow> 'v acc_state \<Rightarrow> nat \<Rightarrow> acc fset \<Rightarrow> ('v acc_state \<times> 'v packet fset)" where
+definition send_1a :: "'v acc_state \<Rightarrow> ('v acc_state \<times> 'v packet fset)" where
   -- {* a tries to become the leader *}
-  "send_1a a s nas acceptors \<equiv>
-    (let
-        b = suc_bal a (ballot s) nas;
+  "send_1a s \<equiv>
+    (let a = id s;
+        b = suc_bal a (ballot s) (nas s);
         msg_1a = Phase1a a b in
-      (s\<lparr>ballot := b\<rparr>, send_all a msg_1a acceptors))"
+      (s\<lparr>ballot := b\<rparr>, send_all a msg_1a s))"
 
-definition receive_1a :: "acc \<Rightarrow> acc \<Rightarrow> bal \<Rightarrow> 'v acc_state \<Rightarrow> ('v acc_state \<times> 'v packet fset)" where
-  "receive_1a a l b s \<equiv>
-    (let bal = ballot s in
+definition receive_1a :: "acc \<Rightarrow> bal \<Rightarrow> 'v acc_state \<Rightarrow> ('v acc_state \<times> 'v packet fset)" where
+  "receive_1a l b s \<equiv>
+    (let a = id s; bal = ballot s in
       (if (bal < b)
        then
           (let
@@ -181,21 +179,21 @@ definition update_onebs ::
   "'v acc_state \<Rightarrow> bal \<Rightarrow> acc \<Rightarrow> (inst \<Rightarrow>f (bal \<times> ('v cmd option))) \<Rightarrow> 'v acc_state" where
   -- {* Update the list of highest voted values when receiving a 1b
     message from a2 for ballot bal containing last_vs *}
-  "update_onebs s bal a2 last_vs \<equiv>
+  "update_onebs s b a last_vs \<equiv>
     let
-      combiner = \<lambda> (xs, y) . (if ((a2, y) \<in> xs) then xs else (insert (a2, y) xs));
-      pair_map = ($ (onebs s $ bal), last_vs $);
+      combiner = \<lambda> (xs, y) . (if (List.member xs (a, y)) then xs else ((a, y) # xs));
+      pair_map = ($ (onebs s $ b), last_vs $);
       at_bal = combiner o$ pair_map
-    in s\<lparr>onebs := (onebs s)(bal $:= at_bal)\<rparr>"
+    in s\<lparr>onebs := (onebs s)(b $:= at_bal)\<rparr>"
 
-definition highest_voted :: "(inst \<Rightarrow>f (acc \<times> bal \<times> ('v cmd option)) set) \<Rightarrow> (inst \<Rightarrow> ('v cmd option))" where
+definition highest_voted :: "(inst \<Rightarrow>f (acc \<times> bal \<times> ('v cmd option)) list) \<Rightarrow> (inst \<Rightarrow> ('v cmd option))" where
   -- {* Makes sense only if no list in the map is empty. *}
   "highest_voted onebs_bal \<equiv>
     let
-        onebs_i = (\<lambda>i. (image (\<lambda>s. snd s) (onebs_bal $ i)));
+        onebs_i = (\<lambda>i. (map (\<lambda>s. snd s) (onebs_bal $ i)));
         (*votes = (map snd) o$ m;
         highest = (\<lambda> l . if (l = []) then None else (fold max l (l!0)) \<bind> (\<lambda> vb . Some (fst vb)))*)
-        highest = (\<lambda>l. if (l = {}) then None else snd (the_elem (Set.bind (Set.filter (\<lambda>le. \<forall>x \<in> l. fst x \<le> fst le) l) (\<lambda>x. {x}))))
+        highest = (\<lambda>bcl. if (bcl = []) then None else snd (fold (\<lambda>bc bc0. if (fst bc0 < fst bc) then bc else bc0) bcl (bcl!0)))
     in highest o onebs_i"
 
 text {* 
@@ -208,60 +206,58 @@ text {*
 
   For now we propose values to all the instances ever started.
 *}
-definition receive_1b :: "acc \<Rightarrow> (inst \<Rightarrow>f (bal \<times> ('v cmd option))) \<Rightarrow> bal \<Rightarrow> acc \<Rightarrow> 'v acc_state \<Rightarrow> nat \<Rightarrow> acc fset \<Rightarrow> ('v acc_state \<times> 'v packet fset)" where
- "receive_1b a last_vs bal a2 s nas acceptors \<equiv> (
+definition receive_1b :: "(inst \<Rightarrow>f (bal \<times> ('v cmd option))) \<Rightarrow> bal \<Rightarrow> acc \<Rightarrow> 'v acc_state \<Rightarrow> ('v acc_state \<times> 'v packet fset)" where
+ "receive_1b last_vs bal a2 s \<equiv> (let a = id s in
     if (bal = ballot s)
     then
       (let s1 = update_onebs s bal a2 last_vs
-       in (if one_b_quorum_received bal s1 nas 
+       in (if one_b_quorum_received bal s1
           then (let
               onebs_bal = onebs s1 $ bal;
-              h = highest_voted onebs_bal;
-              max_i = let l = (finfun_to_list onebs_bal) in (if l = [] then 0 else hd (rev l));
+              highestVoted = highest_voted onebs_bal;
+              max_i = let l = (finfun_to_list onebs_bal) in (if l = [] then 0 else Max (set l));
               s2 = s1\<lparr>leader := True\<rparr>;
               maxInst = (next_inst s2);
               (*Modified*)
-              s3 = s2\<lparr>next_inst := (if max_i+1 < maxInst then maxInst else max_i+1)\<rparr>;
-              twoa_is = [1..<max_i+1];
+              s3 = s2\<lparr>next_inst := (if max_i + 1 < maxInst then maxInst else max_i + 1)\<rparr>;
+              highestDecided = let l = (finfun_to_list (decided s2)) in (if l = [] then 0 else Max (set l));
+              twoa_is = [highestDecided + 1..<max_i+1];
               (* TODO: the following might traverse all the finfun, which is a problem when there are many instances. *)
-              s4 = fold (\<lambda> i s . s\<lparr>twobs := (twobs s)(i $:= ((twobs s $ i)(bal $:= {a})))\<rparr>) twoa_is s3;
-              msgs = map (\<lambda> i . case h i of 
+              s4 = fold (\<lambda> i s . s\<lparr>twobs := (twobs s)(i $:= ((twobs s $ i)(bal $:= [a]))),
+                status := (status s)(i $:= 1)\<rparr>) twoa_is s3;
+              msgs = map (\<lambda> i . case highestVoted i of 
                   None \<Rightarrow> Phase2a i bal NoOp a
                 | Some v \<Rightarrow> Phase2a i bal v a) twoa_is;
-              pckts = map (\<lambda> m . send_all a m acceptors) msgs
+              pckts = map (\<lambda> m . send_all a m s4) msgs
             in (s4, fold (op |\<union>|) pckts {||}) )
           else (s1, {||}) ) )
     else (s, {||}))"
 
 definition is_decided where "is_decided s i \<equiv> decided s $ i \<noteq> None"
 
-definition new_twobs where "new_twobs a ori_twobs \<equiv> insert a ori_twobs"
-
 definition update_twobs where "update_twobs s i b new \<equiv>
   s\<lparr>twobs := (twobs s)(i $:= (twobs s $ i)(b $:= new))\<rparr>"
 
 definition update_decided where 
   "update_decided s i v \<equiv> s\<lparr>
-        decided := (decided s)(i $:= Some v)
+    decided := (decided s)(i $:= Some v), status := (status s)(i $:= 2)
 \<rparr>"
 
-definition receive_2_addl  :: "acc \<Rightarrow> inst \<Rightarrow> bal \<Rightarrow> 'v cmd \<Rightarrow> acc \<Rightarrow> 'v acc_state \<Rightarrow> nat \<Rightarrow> 'v acc_state" where
- "receive_2_addl a i b v l s nas \<equiv>
-    (let ori_twobs = (twobs s $ i $ b) in
-    if (l \<in> ori_twobs) then s 
-     else (let s2 = update_twobs s i b (new_twobs l ori_twobs); votes = (card (twobs s2 $ i $ b))
+definition receive_2_addl  :: "inst \<Rightarrow> bal \<Rightarrow> 'v cmd \<Rightarrow> acc \<Rightarrow> 'v acc_state \<Rightarrow> 'v acc_state" where
+ "receive_2_addl i b v l s \<equiv>
+    (let a = id s; ori_twobs = (twobs s $ i $ b) in
+    if (List.member ori_twobs l) then s 
+     else (let s2 = update_twobs s i b (l#ori_twobs); votes = (length (twobs s2 $ i $ b))
      in (
-          if (2 * votes \<le> nas) (* Build the quorum *)
-          then (
-            (s2)
-          ) else ( 
-              if ( ((nas div 2)+1) = votes) (* Decision Time *)
+          if (2 * votes \<le> (nas s)) (* Build the quorum *)
+          then (s2) else ( 
+              if ( (((nas s) div 2) + 1) = votes) (* Decision Time *)
               then ( 
                (update_decided s2 i v)
               ) else ( 
-                  if (nas = votes) (* Last Message *)
+                  if ((nas s) = votes) (* Last Message *)
                   then ( 
-                    let s3= s2\<lparr>working_instances := (working_instances s)(i $:= 2)\<rparr>
+                    let s3 = s2\<lparr>status := (status s)(i $:= 2)\<rparr>
                     in (s3)
                   ) else (s2) (*extra messages -- but not the last one*)
               )
@@ -269,50 +265,37 @@ definition receive_2_addl  :: "acc \<Rightarrow> inst \<Rightarrow> bal \<Righta
         ))
     )"     
 
-definition receive_2_first  :: "acc \<Rightarrow> inst \<Rightarrow> bal \<Rightarrow> 'v cmd \<Rightarrow> acc \<Rightarrow> 'v acc_state \<Rightarrow> nat \<Rightarrow> 'v acc_state" where
- "receive_2_first a i b v l s nas \<equiv>
-    (let bal = (ballot s); s2 = s\<lparr>vote := (vote s)(i $:= (Some v)),
-                    twobs := (twobs s)(i $:= ((twobs s $ i)(bal $:= {a,l}))),
-                    next_inst := i + 1,
+definition receive_2_first  :: "inst \<Rightarrow> bal \<Rightarrow> 'v cmd \<Rightarrow> acc \<Rightarrow> 'v acc_state \<Rightarrow> 'v acc_state" where
+ "receive_2_first i b v l s \<equiv>
+    (let a = id s; replicaCount = nas s; bal = (ballot s); nextInst = (next_inst s);
+      s2 = s\<lparr>vote := (vote s)(i $:= (Some v)),
+               twobs := (twobs s)(i $:= ((twobs s $ i)(bal $:= [a,l]))),
+                  next_inst := (if (i + 1) < nextInst then nextInst else (i + 1)),
                     last_ballot := (last_ballot s)(i $:= b),(* modified *)
-                    working_instances := (working_instances s)(i $:= 1)\<rparr>
-     in (
-          if (3 < nas)
-          then ( 
-            (s2)
-          ) else ( 
-              if (3 = nas)
-              then ( 
-                (update_decided s2 i v)
-              ) else ( (*nr = 2 *) (*Decided and not working as no more message to receive*)
-                   let s3= s2\<lparr>working_instances := (working_instances s)(i $:= 2)\<rparr> (*This is still working as we have 1 more message to receive *)
-                   in (update_decided s3 i v)
-              )
-          )             
-        )
-     )"
+                      status := (status s)(i $:= 1)\<rparr>
+     in (if (3 = replicaCount) then (update_decided s2 i v) else s2))"
 
 
             
-definition receive_2 :: "acc \<Rightarrow> inst \<Rightarrow> bal \<Rightarrow> 'v cmd \<Rightarrow> acc \<Rightarrow> 'v acc_state \<Rightarrow> nat \<Rightarrow> 'v acc_state" where
-  "receive_2 a i b v l s nas \<equiv>
-  (if ((working_instances s) $ i > 0) (* This is not the first message from the instance *)
+definition receive_2 :: "inst \<Rightarrow> bal \<Rightarrow> 'v cmd \<Rightarrow> acc \<Rightarrow> 'v acc_state \<Rightarrow> 'v acc_state" where
+  "receive_2 i b v l s \<equiv>
+  (if ((status s) $ i > 0) (* This is not the first message from the instance *)
         then (
-          receive_2_addl a i b v l s nas
+          receive_2_addl i b v l s
       ) else (* This is the first message, treat like a propose *)
      (
-          receive_2_first a i b v l s nas
+          receive_2_first i b v l s
      ))"
 
-definition receive_2a :: "acc \<Rightarrow> inst \<Rightarrow> bal \<Rightarrow> 'v cmd \<Rightarrow> acc \<Rightarrow> 'v acc_state \<Rightarrow> nat \<Rightarrow> acc fset \<Rightarrow> ('v acc_state \<times> 'v packet fset)" where
-  "receive_2a a i b v l s nas acceptors \<equiv> (
+definition receive_2a :: "inst \<Rightarrow> bal \<Rightarrow> 'v cmd \<Rightarrow> acc \<Rightarrow> 'v acc_state \<Rightarrow> ('v acc_state \<times> 'v packet fset)" where
+  "receive_2a i b v l s \<equiv> (let a = id s in
   if (ballot s \<le> b) then (* modified *)
-    (receive_2 a i b v l s nas, send_all a (Phase2b i b a v) acceptors)
+    (receive_2 i b v l s, send_all a (Phase2b i b a v) s)
   else
     (s, {||}))"
 
-definition receive_2b :: "acc \<Rightarrow> inst \<Rightarrow> bal \<Rightarrow> acc \<Rightarrow> 'v cmd  \<Rightarrow> 'v acc_state \<Rightarrow> nat \<Rightarrow> ('v acc_state \<times> 'v packet fset)" where
-  "receive_2b a i b a2 v s nas \<equiv> (receive_2 a i b v a2 s nas, {||})"
+definition receive_2b :: "inst \<Rightarrow> bal \<Rightarrow> acc \<Rightarrow> 'v cmd  \<Rightarrow> 'v acc_state \<Rightarrow> ('v acc_state \<times> 'v packet fset)" where
+  "receive_2b i b a2 v s \<equiv> (receive_2 i b v a2 s, {||})"
 
 text {* output transition could return an option *}
 definition learn :: "inst \<Rightarrow> 'v  \<Rightarrow> 'v acc_state \<Rightarrow> ('v acc_state \<times> 'v packet fset) option" where 
@@ -344,25 +327,28 @@ locale mp_ioa = IOA +
     -- {* The number of acceptors *}
 begin
 
+definition mp_acceptors where
+  "mp_acceptors \<equiv> accs nas"
+
 definition mp_asig where
   "mp_asig \<equiv>
-    \<lparr> inputs = { Propose a c | a c . a |\<in>| (mp_acceptors nas)},
-      outputs = { Learn l i v | i v l . l |\<in>| (mp_acceptors nas)},
-      internals = {Receive_fwd a1 a2 v | a1 a2 v . a1 |\<in>| (mp_acceptors nas) \<and> a2 |\<in>| (mp_acceptors nas)}
-        \<union> {Send_1as a | a . a |\<in>| (mp_acceptors nas)}
-        \<union> {Receive_1a_send_1b a1 a2 b | a1 a2 b . a1 |\<in>| (mp_acceptors nas) \<and> a2 |\<in>| (mp_acceptors nas)}
-        \<union> {Receive_1b a1 a2 f b | a1 a2 f b . a1 |\<in>| (mp_acceptors nas) \<and> a2 |\<in>| (mp_acceptors nas)}
-        \<union> {Receive_2a_send_2b a1 a2 i b c | a1 a2 i b c . a1 |\<in>| (mp_acceptors nas) \<and> a2 |\<in>| (mp_acceptors nas)}
-        \<union> {Receive_2b a1 a2 i b c | a1 a2 i b c. a1 |\<in>| (mp_acceptors nas) \<and> a2 |\<in>| (mp_acceptors nas)}
-        \<union> {Learn a i c | a i c . a |\<in>| (mp_acceptors nas)}\<rparr>"
+    \<lparr> inputs = { Propose a c | a c . a |\<in>| mp_acceptors},
+      outputs = { Learn l i v | i v l . l |\<in>| mp_acceptors},
+      internals = {Receive_fwd a1 a2 v | a1 a2 v . a1 |\<in>| mp_acceptors \<and> a2 |\<in>| mp_acceptors}
+        \<union> {Send_1as a | a . a |\<in>| mp_acceptors}
+        \<union> {Receive_1a_send_1b a1 a2 b | a1 a2 b . a1 |\<in>| mp_acceptors \<and> a2 |\<in>| mp_acceptors}
+        \<union> {Receive_1b a1 a2 f b | a1 a2 f b . a1 |\<in>| mp_acceptors \<and> a2 |\<in>| mp_acceptors}
+        \<union> {Receive_2a_send_2b a1 a2 i b c | a1 a2 i b c . a1 |\<in>| mp_acceptors \<and> a2 |\<in>| mp_acceptors}
+        \<union> {Receive_2b a1 a2 i b c | a1 a2 i b c. a1 |\<in>| mp_acceptors \<and> a2 |\<in>| mp_acceptors}
+        \<union> {Learn a i c | a i c . a |\<in>| mp_acceptors}\<rparr>"
 
 fun init_nodes_state::"nat \<Rightarrow> nat \<Rightarrow>f 'a acc_state" where
-  "init_nodes_state (0::nat) = (K$ init_acc_state)"
-| "init_nodes_state (Suc i) = (init_nodes_state i)(i $:= init_acc_state)"
+  "init_nodes_state (0::nat) = (K$ (init_acc_state nas 0))"
+| "init_nodes_state (Suc i) = (init_nodes_state i)(i $:= (init_acc_state nas i))"
 
 lemma init_acc: 
 assumes "a \<ge> 0"
-shows "(init_nodes_state (Suc a)) $ a = init_acc_state" using assms
+shows "(init_nodes_state (Suc a)) $ a = (init_acc_state nas a)" using assms
 by (induct a rule:init_nodes_state.induct, auto)
 
 definition mp_start where
@@ -373,21 +359,21 @@ definition update_state where
     s\<lparr>node_states := (node_states s)(a $:= a_s),
       network := network s |\<union>| packets\<rparr>"
 
-fun mp_transit where
+(*fun mp_transit where
   "mp_transit s (Receive_fwd src dest v) = (if Packet src dest (Fwd v) |\<in>| network s 
-    then (let (new_s, ps) = receive_fwd dest v (node_states s $ dest) nas (mp_acceptors nas) in 
+    then (let (new_s, ps) = receive_fwd dest v (node_states s $ dest) nas mp_acceptors in 
       update_state dest new_s ps s)
     else s)"
-|  "mp_transit s (Propose a (Cmd v)) = (let (new_s, ps) = propose a v (node_states s $ a) nas (mp_acceptors nas) in
+|  "mp_transit s (Propose a (Cmd v)) = (let (new_s, ps) = propose a v (node_states s $ a) nas mp_acceptors in
     update_state a new_s ps s)" 
 | "mp_transit s (Receive_1a_send_1b src dest b) = (if (Packet src dest (Phase1a src b) |\<in>| network s) 
     then let (new_s, ps) = receive_1a dest src b (node_states s $ dest) in
       update_state dest new_s ps s 
     else s)"
-| "mp_transit s (Send_1as l) = (let (new_s, ps) = send_1a l (node_states s $ l) nas (mp_acceptors nas) in
+| "mp_transit s (Send_1as l) = (let (new_s, ps) = send_1a l (node_states s $ l) nas mp_acceptors in
     update_state l new_s ps s)"
 | "mp_transit s (Receive_1b src l vs b) = (if (Packet src l (Phase1b vs b src) |\<in>| network s)
-    then let (new_s, ps) = receive_1b l vs b src (node_states s $ l) nas (mp_acceptors nas) in
+    then let (new_s, ps) = receive_1b l vs b src (node_states s $ l) nas mp_acceptors in
       update_state l new_s ps s 
     else s)"
 | "mp_transit s (Receive_2b a l i b cm) = (if (Packet a l (Phase2b i b a cm) |\<in>| network s)
@@ -395,15 +381,15 @@ fun mp_transit where
       update_state l new_s ps s 
     else s)"
 | "mp_transit s (Receive_2a_send_2b l dest i b cm) = (if (Packet l dest (Phase2a i b cm l) |\<in>| network s)
-    then (let (new_s, ps) = receive_2a dest i b cm l (node_states s $ dest) nas (mp_acceptors nas) in
+    then (let (new_s, ps) = receive_2a dest i b cm l (node_states s $ dest) nas mp_acceptors in
         update_state dest new_s ps s)
     else s)"
 | "mp_transit s (Learn a i (Cmd v)) = (case (learn i v (node_states s $ a)) of (Some st) \<Rightarrow> 
-  (let (new_s, ps) = st in update_state a new_s ps s)| None \<Rightarrow> s)"
+  (let (new_s, ps) = st in update_state a new_s ps s)| None \<Rightarrow> s)"*)
 
 end
 
-global_interpretation mp_ioa_3:mp_ioa "3"
+(*global_interpretation mp_ioa_3:mp_ioa "3"
 defines mp_start = mp_ioa_3.mp_start and mp_transit = mp_ioa_3.mp_transit
 done
 
@@ -418,9 +404,6 @@ definition safe_at::"'v mp_state \<Rightarrow> inst \<Rightarrow> nat \<Rightarr
       Some cm \<Rightarrow> (
         case (decided ((node_states s) $ acc\<^sub>2) $ i) of None \<Rightarrow> True |
           Some cs \<Rightarrow> (cm = cs))))"
-
-definition get_decided::"'v mp_state \<Rightarrow> acc \<Rightarrow> inst \<Rightarrow> 'v cmd option" where
-  "get_decided s acc i \<equiv> (decided ((node_states s) $ acc) $ i)"
 
 definition ballot_constraint where
   "ballot_constraint s bound \<equiv>
@@ -444,9 +427,12 @@ definition inst_constraint where
       inst_list_sorted = sort inst_list;
       max_inst = if inst_list_sorted = [] then 1 else inst_list_sorted ! (length inst_list_sorted - 1)
     in
-    max_inst \<le> bound"
+    max_inst \<le> bound"*)
 
 subsection {* Code generation *}
+
+definition get_decided::"'v mp_state \<Rightarrow> acc \<Rightarrow> inst \<Rightarrow> 'v cmd option" where
+  "get_decided s acc i \<equiv> (decided ((node_states s) $ acc) $ i)"
 
 text {* We need to rename a few modules to let the Scala compiler resolve circular dependencies. *}
 code_identifier
@@ -476,8 +462,14 @@ code_identifier
 | code_module Complete_Partial_Order \<rightharpoonup> (Scala) MicroCheckerLib
 | code_module Lattices \<rightharpoonup> (Scala) MicroCheckerLib
 
-export_code learn send_1a propose init_acc_state get_ballot is_leader get_leader
-mp_ioa_3.mp_start mp_ioa_3.mp_transit safe_at get_decided ballot_constraint inst_constraint
-   in Scala file "MultiPaxos4.scala"
+fun processExternalEvent where
+  "processExternalEvent (Phase1a l b) s = receive_1a l b s"
+| "processExternalEvent (Phase1b last_vote b a) s = receive_1b last_vote b a s "
+| "processExternalEvent (Phase2a i b cm l) s = receive_2a i b cm l s"
+| "processExternalEvent (Phase2b i b a cm) s = receive_2b i b a cm s"
+| "processExternalEvent (Fwd v) s = receive_fwd v s"
+
+export_code learn send_1a propose init_acc_state get_ballot is_leader get_leader 
+  get_decided propose processExternalEvent in Scala file "MultiPaxos4.scala"
 
 end
